demo/utod/DemoSpec.v
@@ -10,7 +10,7 @@ Require Import DemoHeader.
 
 Set Implicit Arguments.
 
-Local Obligation Tactic := ii; ss; des; inv_all_once; ss; clarify.
+Local Obligation Tactic := ii; ss; des; inv_all_once; repeat des_u; ss; clarify.
 
 Section MODSEM.
 
@@ -20,6 +20,7 @@ Section MODSEM.
        prog_public := [func_id; main_id];
        prog_main := main_id |}.
 
+  Variable midx: Midx.t.
   Variable skenv_link: SkEnv.t.
   Variable p: unit.
   Let skenv: SkEnv.t := (SkEnv.project skenv_link) (Sk.of_program id prog).
@@ -48,13 +49,14 @@ Section MODSEM.
       ModSem.state := state;
       ModSem.genvtype := unit;
       ModSem.step := bot5;
-      ModSem.at_external := bot2;
-      ModSem.initial_frame := initial_frame;
-      ModSem.final_frame := final_frame;
-      ModSem.after_external := bot3;
+      ModSem.at_external := bot3;
+      ModSem.initial_frame := coerce initial_frame;
+      ModSem.final_frame := coerce final_frame;
+      ModSem.after_external := bot4;
       ModSem.globalenv := tt;
       ModSem.skenv := skenv;
       ModSem.skenv_link := skenv_link;
+      ModSem.midx := midx;
     |}
   .
 
