Makefile
@@ -1,11 +1,6 @@
 COQMODULE    := compcomp
 # COQTHEORIES  := $(wildcard */*.v) #*/*.v
-# COQTHEORIES  := $(shell find . -iname '*.v')
-COQTHEORIES_ := $(shell find . -type d \( -path ./bound -o -path ./selfsim -o -path ./demo -o -path ./backend -o -path ./x86 -o -path ./cfrontend -o -path ./driver \) -prune -o -iname '*.v') \
-	./backend/RenumberproofC.v ./backend/RTLC.v ./backend/SeparationC.v \
-	./backend/InliningproofC.v ./backend/ValueAnalysisC.v ./backend/ValueDomainC.v
-COQTHEORIES  := $(filter-out ./proof/StoreArgumentsProps.v ./proof/MatchSimModSemSR.v ./proof/SimModSemSR.v,$(COQTHEORIES_))
-
+COQTHEORIES  := $(shell find . -iname '*.v')
 
 .PHONY: all proof proof-quick graph
 
